current equation:
$$
\lambda A^2\alpha \beta(\alpha-1)(\beta-1)x^{2(\alpha-1)}y^{2(\beta-1)}-\lambda^2A^2\alpha^2\beta^2x^{2(\alpha-1)}y^{2(\beta-1)}
$$
sneaky rearrange:
$$
\lambda A^2 x^{2(\alpha-1)}y^{2(\beta-1)}\alpha \beta(\alpha-1)(\beta-1)-\lambda A^2 x^{2(\alpha-1)}y^{2(\beta-1)}\alpha^2\beta^2
$$
here, there's a common factor of $\lambda A^2 x^{2(\alpha-1)}y^{2(\beta-1)}$. This allows you to factor it out and you're left with:
$$
\lambda A^2 x^{2(\alpha-1)}y^{2(\beta-1)}[\alpha \beta (\alpha-1)(\beta-1) - \alpha^2 \beta^2]
$$
